{-# OPTIONS --type-in-type #-}
module Poly.Monoidal.Coproduct where

--------------------------------------------------------------------------------

open import Data.Product using (_,_; âˆƒ-syntax)
open import Data.Sum using (_âŠ_; injâ‚; injâ‚‚)
open import Data.Unit
open import Poly
open import Poly.Comonoid
open import Poly.Monoid
open import Poly.Isomorphism
open import Poly.SetFunctor

open ProposedIso
open _â‰ƒ_

--------------------------------------------------------------------------------

-- | P + Q
-- The Categorical Co-Product of two Polyonomials
--
-- P + Q â‰” âˆ‘[ j âˆˆ I ] x^aáµ¢ + âˆ‘[ j âˆˆ J ] y^bâ±¼
infixr 6 _+_
_+_ : Poly â†’ Poly â†’ Poly
(P + Q) .Base = P .Base âŠ Q .Base
(P + Q) .Fiber (injâ‚ x) = P .Fiber x
(P + Q) .Fiber (injâ‚‚ y) = Q .Fiber y

_+â‡’_ : âˆ€{P Q R Z : Poly} â†’ P â‡’ Q â†’ R â‡’ Z â†’ P + R â‡’ Q + Z
(pâ‡’q +â‡’ râ‡’z) .map-base (injâ‚ ptag) = injâ‚ (map-base pâ‡’q ptag)
(pâ‡’q +â‡’ râ‡’z) .map-base (injâ‚‚ rtag) = injâ‚‚ (map-base râ‡’z rtag)
(pâ‡’q +â‡’ râ‡’z) .map-fiber (injâ‚ ptag) = map-fiber pâ‡’q ptag
(pâ‡’q +â‡’ râ‡’z) .map-fiber (injâ‚‚ rtag) = map-fiber râ‡’z rtag

+-split-l : âˆ€{P : Poly} â†’ P â‡’ P + P
map-base +-split-l p-base = injâ‚ p-base
map-fiber +-split-l p-base p-fib = p-fib

+-split-r : âˆ€{P : Poly} â†’ P â‡’ P + P
map-base +-split-r p-base = injâ‚‚ p-base
map-fiber +-split-r p-base p-fib = p-fib

+-monoid : âˆ€{P : Poly} â†’ ProposedMonoid (_+_) ğŸ˜
ProposedMonoid.P (+-monoid {P}) = P
map-base (Îµ (+-monoid {P})) ()
map-fiber (Îµ (+-monoid {P})) () _
map-base (_â‹†_ (+-monoid {P})) (injâ‚ p-base) = p-base
map-base (_â‹†_ (+-monoid {P})) (injâ‚‚ p-base) = p-base
map-fiber (_â‹†_ (+-monoid {P})) (injâ‚ p-base) p-fib = p-fib
map-fiber (_â‹†_ (+-monoid {P})) (injâ‚‚ p-base) p-fib = p-fib

+-unital-r : âˆ€{P : Poly} â†’ ProposedIso (P + ğŸ˜) P
map-base (fwd +-unital-r) (injâ‚ p-base) = p-base
map-fiber (fwd +-unital-r) (injâ‚ p-base) p-fib = p-fib
map-base (bwd +-unital-r) p-base = injâ‚ p-base
map-fiber (bwd +-unital-r) p-base p-fib = p-fib

+-unital-l : âˆ€{P : Poly} â†’ ProposedIso (ğŸ˜ + P) P
map-base (fwd +-unital-l) (injâ‚‚ p-base) = p-base
map-fiber (fwd +-unital-l) (injâ‚‚ p-base) p-fib = p-fib
map-base (bwd +-unital-l) p-base = injâ‚‚ p-base
map-fiber (bwd +-unital-l) p-base p-fib = p-fib

-- | Co-Product Left Inclusion
leftâ‚š : âˆ€{P Q : Poly} â†’ P â‡’ (P + Q) 
leftâ‚š = +-unital-r .bwd â¨Ÿâ‚š idâ‚š +â‡’ +-monoid .Îµ

-- | Co-Product Right Inclusion
rightâ‚š : âˆ€{P Q : Poly} â†’ Q â‡’ (P + Q)
rightâ‚š = +-unital-l .bwd â¨Ÿâ‚š +-monoid .Îµ +â‡’ idâ‚š

-- | Co-Product eliminator
eitherâ‚š : âˆ€{P Q R : Poly} â†’ P â‡’ R â†’ Q â‡’ R â†’ (P + Q) â‡’ R
eitherâ‚š pâ‡’r qâ‡’r .map-base (injâ‚ ptag) = pâ‡’r .map-base ptag
eitherâ‚š pâ‡’r qâ‡’r .map-base (injâ‚‚ qtag) = qâ‡’r .map-base qtag
eitherâ‚š pâ‡’r qâ‡’r .map-fiber (injâ‚ tag) = pâ‡’r .map-fiber tag
eitherâ‚š pâ‡’r qâ‡’r .map-fiber (injâ‚‚ tag) = qâ‡’r .map-fiber tag

+-left : âˆ€{P Q R : Poly} â†’ P â‡’ Q â†’ (P + R) â‡’ (Q + R)
+-left pâ‡’q .map-base (injâ‚ ptag) = injâ‚ (map-base pâ‡’q ptag)
+-left pâ‡’q .map-base (injâ‚‚ rtag) = injâ‚‚ rtag
+-left pâ‡’q .map-fiber (injâ‚ ptag) args = map-fiber pâ‡’q ptag args
+-left pâ‡’q .map-fiber (injâ‚‚ rtag) args = args

right : âˆ€{P Q R : Poly} â†’ P â‡’ Q â†’ (R + P) â‡’ (R + Q)
right pâ‡’q .map-base (injâ‚ rtag) = injâ‚ rtag
right pâ‡’q .map-base (injâ‚‚ ptag) = injâ‚‚ (map-base pâ‡’q ptag)
right pâ‡’q .map-fiber (injâ‚ rtag) args = args
right pâ‡’q .map-fiber (injâ‚‚ ptag) args = map-fiber pâ‡’q ptag args

-- | Index sums
Sum : (I : Set) â†’ (I â†’ Poly) â†’ Poly
Sum I P .Base = âˆƒ[ i ] P i .Base
Sum I P .Fiber (i , ptag) = P i .Fiber ptag

infix 2 Sum
syntax Sum I (Î» i â†’ P) = Î£â‚š[ i âˆˆ I ] P

âŸ¦âŸ§-+ : âˆ€{P Q : Poly} â†’ âŸ¦ P + Q âŸ§ â‰ƒ âŸ¦ P âŸ§ +â‚ âŸ¦ Q âŸ§
âŸ¦âŸ§-+ .to (injâ‚ ptag , x) = injâ‚ (ptag , x)
âŸ¦âŸ§-+ .to (injâ‚‚ qtag , y) = injâ‚‚ (qtag , y)
âŸ¦âŸ§-+ .from (injâ‚ (ptag , x)) = injâ‚ ptag , x
âŸ¦âŸ§-+ .from (injâ‚‚ (qtag , y)) = injâ‚‚ qtag , y

âŸ¦âŸ§-Sum : {I : Set} â†’ {P : I â†’ Poly} â†’ âŸ¦ Î£â‚š[ i âˆˆ I ] (P i) âŸ§ â‰ƒ (Î£â‚[ i âˆˆ I ] âŸ¦ P i âŸ§)
âŸ¦âŸ§-Sum .to ((i , ptag) , f) = i , ptag , f
âŸ¦âŸ§-Sum .from (i , ptag , f) = (i , ptag) , f
